Rename conversion function
Old name: inject, new name: convert

arrays/CommutingCanonicalArrImpl.v
@@ -13,30 +13,30 @@ Module CommutingCanonicalArrayImpl (N : VerifiedNaturalInterface)
   Definition set := Canon.set.
   Definition concat := Canon.concat.
 
-  Definition inject A (m:M A) := m.
+  Definition convert A (m:M A) := m.
 
   Lemma make_commutes : forall (A : Type) n (x : A),
-      inject (make n x) = Canon.make n x.
+      convert (make n x) = Canon.make n x.
     auto.
   Defined.
 
   Lemma len_commutes : forall (A : Type) (l : M A),
-      len l =  Canon.len (inject l).
+      len l =  Canon.len (convert l).
     auto.
   Defined.
 
   Lemma get_commutes : forall A (l : M A) index,
-      get l index = Canon.get (inject l) index.
+      get l index = Canon.get (convert l) index.
     auto.
   Defined.
 
   Lemma set_commutes : forall A (l : M A) index x,
-      inject (set l index x) = Canon.set (inject l) index x.
+      convert (set l index x) = Canon.set (convert l) index x.
     auto.
   Defined.
 
   Lemma concat_commutes : forall A (l : M A) (l' : M A),
-      inject (concat l l') = Canon.concat (inject l) (inject l').
+      convert (concat l l') = Canon.concat (convert l) (convert l').
     auto.
   Defined.
 End CommutingCanonicalArrayImpl.
