arrays/VerifiedArrayIntf.v
@@ -14,23 +14,23 @@ Module Type VerifiedArrayInterface (N:VerifiedNaturalInterface)
   Parameter set : forall A : Type, M A -> N.N -> A -> M A.
   Parameter concat : forall A : Type, M A -> M A -> M A.
 
-  Parameter inject : forall A : Type, M A -> list A.
+  Parameter convert : forall A : Type, M A -> list A.
 
   Module Canon := CanonicalArrayImpl N.
 
   Axiom make_commutes : forall (A : Type) n (x : A),
-    inject (make n x) = Canon.make n x.
+    convert (make n x) = Canon.make n x.
   Axiom len_commutes : forall (A : Type) (l : M A),
-    len l =  Canon.len (inject l).
+    len l =  Canon.len (convert l).
   Axiom get_commutes : forall A (l : M A) index,
-    get l index = Canon.get (inject l) index.
+    get l index = Canon.get (convert l) index.
   Axiom set_commutes : forall A (l : M A) index x,
-    inject (set l index x) = Canon.set (inject l) index x.
+    convert (set l index x) = Canon.set (convert l) index x.
   Axiom concat_commutes : forall A (l : M A) (l' : M A),
-    inject (concat l l') = Canon.concat (inject l) (inject l').
+    convert (concat l l') = Canon.concat (convert l) (convert l').
 
   Axiom concat_assoc : forall A (l1 l2 l3 : M A),
-    inject (concat (concat l1 l2) l3) = inject (concat l1 (concat l2 l3)).
+    convert (concat (concat l1 l2) l3) = convert (concat l1 (concat l2 l3)).
 End VerifiedArrayInterface.
 
 Module VerifiedCommutingArrayInterface (N:VerifiedNaturalInterface)
@@ -42,7 +42,7 @@ Module VerifiedCommutingArrayInterface (N:VerifiedNaturalInterface)
   Definition get := A.get.
   Definition set := A.set.
   Definition concat := A.concat.
-  Definition inject := A.inject.
+  Definition convert := A.convert.
 
   Module Canon := A.Canon.
 
@@ -53,7 +53,7 @@ Module VerifiedCommutingArrayInterface (N:VerifiedNaturalInterface)
   Definition concat_commutes := A.concat_commutes.
 
   Lemma concat_assoc : forall A (l1 l2 l3 : M A),
-      inject (concat (concat l1 l2) l3) = inject (concat l1 (concat l2 l3)).
+      convert (concat (concat l1 l2) l3) = convert (concat l1 (concat l2 l3)).
     intros A l1 l2 l3.
     rewrite A.concat_commutes.
     rewrite A.concat_commutes.
