naturals/VerifiedNatIntf.v
@@ -10,20 +10,20 @@ Module Type VerifiedNaturalInterface <: CommutingNaturalInterface.
   Parameter add : N -> N -> N.
   Parameter sub : N -> N -> N.
   Parameter comp : N -> N -> comparison.
-  Parameter inject : N -> nat.
+  Parameter convert : N -> nat.
 
-  Axiom injective : forall n n' : N, inject n = inject n' -> n = n'.
-  Axiom zero_commutes : inject zero = CanonicalNaturalImpl.zero.
+  Axiom convert_injective : forall n n' : N, convert n = convert n' -> n = n'.
+  Axiom zero_commutes : convert zero = CanonicalNaturalImpl.zero.
   Axiom succ_commutes : forall n : N,
-    inject (succ n) = CanonicalNaturalImpl.succ (inject n).
+    convert (succ n) = CanonicalNaturalImpl.succ (convert n).
   Axiom pred_commutes : forall n : N,
-    inject (pred n) = CanonicalNaturalImpl.pred (inject n).
+    convert (pred n) = CanonicalNaturalImpl.pred (convert n).
   Axiom add_commutes : forall n n' : N,
-    inject (add n n') = CanonicalNaturalImpl.add (inject n) (inject n').
+    convert (add n n') = CanonicalNaturalImpl.add (convert n) (convert n').
   Axiom sub_commutes : forall n n' : N,
-    inject (sub n n') = CanonicalNaturalImpl.sub (inject n) (inject n').
+    convert (sub n n') = CanonicalNaturalImpl.sub (convert n) (convert n').
   Axiom comp_commutes : forall n n' : N,
-    comp n n' = CanonicalNaturalImpl.comp (inject n) (inject n').
+    comp n n' = CanonicalNaturalImpl.comp (convert n) (convert n').
 
   Axiom pos_succ : forall (n:N), comp n zero = Gt -> exists n', n = succ n'.
   Axiom pred_succ : forall (n:N), pred (succ n) = n.
@@ -50,8 +50,8 @@ Module VerifiedCommutingNaturalImpl (C : CommutingNaturalInterface) : VerifiedNa
   Definition add := C.add.
   Definition sub := C.sub.
   Definition comp := C.comp.
-  Definition inject := C.inject.
-  Definition injective := C.injective.
+  Definition convert := C.convert.
+  Definition convert_injective := C.convert_injective.
   Definition zero_commutes := C.zero_commutes.
   Definition succ_commutes := C.succ_commutes.
   Definition pred_commutes := C.pred_commutes.
@@ -64,7 +64,7 @@ Module VerifiedCommutingNaturalImpl (C : CommutingNaturalInterface) : VerifiedNa
     intros n.
     rewrite comp_commutes.
     rewrite zero_commutes.
-    remember (C.inject n) as m.
+    remember (C.convert n) as m.
     destruct m;
         symmetry in Heqm; simpl.
       (* 0 *)
@@ -72,7 +72,7 @@ Module VerifiedCommutingNaturalImpl (C : CommutingNaturalInterface) : VerifiedNa
       (* S m *)
       intros _.
       refine (ex_intro _ (pred n) _).
-        apply C.injective.
+        apply C.convert_injective.
         rewrite succ_commutes.
         rewrite pred_commutes.
         rewrite Heqm.
@@ -82,7 +82,7 @@ Module VerifiedCommutingNaturalImpl (C : CommutingNaturalInterface) : VerifiedNa
 
   Lemma pred_succ : forall (n:N), pred (succ n) = n.
     intros n.
-    apply C.injective.
+    apply C.convert_injective.
     rewrite C.pred_commutes.
     rewrite C.succ_commutes.
     auto.
@@ -90,7 +90,7 @@ Module VerifiedCommutingNaturalImpl (C : CommutingNaturalInterface) : VerifiedNa
 
   Lemma add_zero : forall (n:N), add C.zero n = n.
     intros n.
-    apply (C.injective).
+    apply C.convert_injective.
     rewrite (C.add_commutes _ _).
     rewrite (C.zero_commutes).
     auto.
@@ -98,7 +98,7 @@ Module VerifiedCommutingNaturalImpl (C : CommutingNaturalInterface) : VerifiedNa
 
   Lemma add_succ : forall (m n : N), add (succ m) n = succ (add m n).
     intros m n.
-    apply (C.injective).
+    apply C.convert_injective.
     rewrite (C.add_commutes _ _).
     rewrite (C.succ_commutes _).
     rewrite (C.succ_commutes _).
@@ -110,7 +110,7 @@ Module VerifiedCommutingNaturalImpl (C : CommutingNaturalInterface) : VerifiedNa
   Lemma add_succ_right : forall (m n : N),
       add m (succ n) = add (succ m) n.
     intros m n.
-    apply (C.injective).
+    apply C.convert_injective.
     rewrite (C.add_commutes _ _).
     rewrite (C.succ_commutes _).
     rewrite (C.add_commutes _ _).
@@ -121,15 +121,15 @@ Module VerifiedCommutingNaturalImpl (C : CommutingNaturalInterface) : VerifiedNa
 
   Lemma sub_zero : forall (n : N), sub n C.zero = n.
     intros n.
-    apply C.injective.
+    apply C.convert_injective.
     rewrite (C.sub_commutes _ _).
     rewrite C.zero_commutes.
-    destruct (C.inject n); auto.
+    destruct (C.convert n); auto.
   Defined.
 
   Lemma sub_succ : forall (m n:N), sub (succ m) (succ n) = sub m n.
     intros m n.
-    apply C.injective.
+    apply C.convert_injective.
     rewrite C.sub_commutes.
     rewrite C.sub_commutes.
     rewrite C.succ_commutes.
@@ -139,12 +139,12 @@ Module VerifiedCommutingNaturalImpl (C : CommutingNaturalInterface) : VerifiedNa
 
   Lemma sub_pred : forall (m n:N), sub (pred m) n = sub m (succ n).
     intros m n.
-    apply C.injective.
+    apply C.convert_injective.
     rewrite C.sub_commutes.
     rewrite C.sub_commutes.
     rewrite C.pred_commutes.
     rewrite C.succ_commutes.
-    destruct (C.inject m);
+    destruct (C.convert m);
       simpl; reflexivity.
   Defined.
 
@@ -152,7 +152,7 @@ Module VerifiedCommutingNaturalImpl (C : CommutingNaturalInterface) : VerifiedNa
     intros n.
     rewrite C.comp_commutes.
     rewrite C.zero_commutes.
-    destruct (C.inject n);
+    destruct (C.convert n);
       simpl; congruence.
   Defined.
 
@@ -171,7 +171,7 @@ Module VerifiedCommutingNaturalImpl (C : CommutingNaturalInterface) : VerifiedNa
       (* -> *)
       rewrite (C.comp_commutes _ _).
       intros Hcomp.
-      apply C.injective.
+      apply C.convert_injective.
       apply (CanonicalNatImpl.comp_eq).
       assumption.
       (* <- *)
