arrays/CommutingArrayIntf.v
@@ -14,20 +14,20 @@ Module Type CommutingArrayInterface (N : VerifiedNaturalInterface) <: ArrayInter
   Parameter set : forall A, M A -> N.N -> A -> M A.
   Parameter concat : forall A, M A -> M A -> M A.
 
-  Parameter inject : forall A : Type, M A -> Canon.M A.
+  Parameter convert : forall A : Type, M A -> Canon.M A.
 
   Axiom make_commutes : forall (A : Type) n (x : A),
-    inject (make n x) = Canon.make n x.
+    convert (make n x) = Canon.make n x.
 
   Axiom len_commutes : forall (A : Type) (l : M A),
-    len l =  Canon.len (inject l).
+    len l =  Canon.len (convert l).
 
   Axiom get_commutes : forall A (l : M A) index,
-    get l index = Canon.get (inject l) index.
+    get l index = Canon.get (convert l) index.
 
   Axiom set_commutes : forall A (l : M A) index x,
-    inject (set l index x) = Canon.set (inject l) index x.
+    convert (set l index x) = Canon.set (convert l) index x.
 
   Axiom concat_commutes : forall A (l : M A) (l' : M A),
-    inject (concat l l') = Canon.concat (inject l) (inject l').
+    convert (concat l l') = Canon.concat (convert l) (convert l').
 End CommutingArrayInterface.
